Congruence_Closure_Explain/CC_Definition.thy
@@ -1,7 +1,6 @@
 chapter \<open>Congruence Closure Algorithm with Explain Operation\<close>
 theory CC_Definition
-  imports 
-    "../Union_Find_Explain/Explain_Correctness" 
+  imports "../Union_Find_Explain/Explain_Correctness"
 begin
 
 section \<open>Definitions\<close>
@@ -17,11 +16,13 @@ text \<open>The input equations to this congruence closure algorithm need
 
       For example the equation \<open>2 \<approx> 5\<close> should be interpreted as \<open>c\<^sub>2 = c\<^sub>5\<close>.\<close>
 
-datatype equation = Constants nat nat ("_ \<approx> _" 51)
-  | Function nat nat nat                 ("F _ _ \<approx> _" 51)
+datatype equation =
+  Constants nat nat ("_ \<approx> _" 51)
+| Function nat nat nat ("F _ _ \<approx> _" 51)
 
-datatype pending_equation = One equation
-  | Two equation equation
+datatype pending_equation =
+  One equation
+| Two equation equation
 
 term "a \<approx> b"
 term "if (F a b \<approx> c) = F a b \<approx> c then False else True"
@@ -41,7 +42,7 @@ text \<open>Data structure for the congruence closure operations (merge, are_con
   \<open>pf_labels\<close>: for each edge in the \<open>proof_forest\<close>, a label with the input equations
   \<open>input\<close>: a set of the input equation, useful for proofs
 \<close>
-record congruence_closure =
+record cc_state =
   cc_list :: "nat list"
   use_list :: "equation list list"
   lookup :: "equation option list list"
@@ -51,172 +52,171 @@ record congruence_closure =
   input :: "equation set"
 
 text \<open>For updating two dimensional lists.\<close>
-abbreviation upd :: "'a list list \<Rightarrow> nat \<Rightarrow> nat \<Rightarrow> 'a \<Rightarrow> 'a list list"
-  where 
+abbreviation upd :: "'a list list \<Rightarrow> nat \<Rightarrow> nat \<Rightarrow> 'a \<Rightarrow> 'a list list" where 
 "upd xs n m e \<equiv> xs[n := (xs ! n)[m := e]]"
 
 text \<open>Finds the entry in the lookup table for the representatives of \<open>a\<^sub>1\<close> and \<open>a\<^sub>2\<close>.\<close>
-abbreviation lookup_entry :: "equation option list list \<Rightarrow> nat list \<Rightarrow> nat \<Rightarrow> nat \<Rightarrow> equation option"
-  where
-"lookup_entry t l a\<^sub>1 a\<^sub>2 \<equiv> t ! rep_of l a\<^sub>1 ! rep_of l a\<^sub>2"
+abbreviation lookup_entry ::
+  "equation option list list \<Rightarrow> nat list \<Rightarrow> nat \<Rightarrow> nat \<Rightarrow> equation option" where
+  "lookup_entry t l a\<^sub>1 a\<^sub>2 \<equiv> t ! rep_of l a\<^sub>1 ! rep_of l a\<^sub>2"
 
-fun lookup_Some :: "equation option list list \<Rightarrow> nat list \<Rightarrow> equation \<Rightarrow> bool"
-  where
-"lookup_Some t l (F a\<^sub>1 a\<^sub>2 \<approx> a) = (\<not>Option.is_none (lookup_entry t l a\<^sub>1 a\<^sub>2))"
-| "lookup_Some t l (a \<approx> b) = False"
+fun lookup_Some :: "equation option list list \<Rightarrow> nat list \<Rightarrow> equation \<Rightarrow> bool" where
+  "lookup_Some t l (F a\<^sub>1 a\<^sub>2 \<approx> a) \<longleftrightarrow> \<not> Option.is_none (lookup_entry t l a\<^sub>1 a\<^sub>2)"
+| "lookup_Some t l (a \<approx> b) \<longleftrightarrow> False"
 
 \<comment> \<open>Should only be used if \<open>lookup(a\<^sub>1, a\<^sub>2)\<close> is not None and if the equation is not of the type (a = b)\<close>
-fun link_to_lookup :: "equation option list list \<Rightarrow> nat list \<Rightarrow> equation \<Rightarrow> pending_equation"
-  where
-"link_to_lookup t l (F a\<^sub>1 a\<^sub>2 \<approx> a) = Two (F a\<^sub>1 a\<^sub>2 \<approx> a) (the (lookup_entry t l a\<^sub>1 a\<^sub>2))"
+fun link_to_lookup :: "equation option list list \<Rightarrow> nat list \<Rightarrow> equation \<Rightarrow> pending_equation" where
+  "link_to_lookup t l (F a\<^sub>1 a\<^sub>2 \<approx> a) = Two (F a\<^sub>1 a\<^sub>2 \<approx> a) (the (lookup_entry t l a\<^sub>1 a\<^sub>2))"
   \<comment> \<open>This should not be invoked.\<close>
 | "link_to_lookup t l (a \<approx> b) = One (a \<approx> b)"
 
 \<comment> \<open>Should only be used if \<open>lookup(a\<^sub>1, a\<^sub>2)\<close> is not None and if the equation is not of the type (a = b)\<close>
 fun update_lookup :: "equation option list list \<Rightarrow> nat list \<Rightarrow> equation \<Rightarrow> equation option list list"
   where
-"update_lookup t l (F c\<^sub>1 c\<^sub>2 \<approx> c) = upd t (rep_of l c\<^sub>1) (rep_of l c\<^sub>2) (Some (F c\<^sub>1 c\<^sub>2 \<approx> c))"
+  "update_lookup t l (F c\<^sub>1 c\<^sub>2 \<approx> c) = upd t (rep_of l c\<^sub>1) (rep_of l c\<^sub>2) (Some (F c\<^sub>1 c\<^sub>2 \<approx> c))"
   \<comment> \<open>This should not be invoked.\<close>
 | "update_lookup t l (a \<approx> b) = t"
 
-fun left :: "pending_equation \<Rightarrow> nat"
-  where
-"left (One (a \<approx> b)) = a"
+fun left :: "pending_equation \<Rightarrow> nat" where
+  "left (One (a \<approx> b)) = a"
 | "left (Two (F a\<^sub>1 a\<^sub>2 \<approx> a) (F b\<^sub>1 b\<^sub>2 \<approx> b)) = a"
   \<comment> \<open>This should not be invoked.\<close>
 | "left a = undefined"
 
-fun right :: "pending_equation \<Rightarrow> nat"
-  where
-"right (One (a \<approx> b)) = b"
+fun right :: "pending_equation \<Rightarrow> nat" where
+  "right (One (a \<approx> b)) = b"
 | "right (Two (F a\<^sub>1 a\<^sub>2 \<approx> a) (F b\<^sub>1 b\<^sub>2 \<approx> b)) = b"
   \<comment> \<open>This should not be invoked.\<close>
 | "right a = undefined"
 
 text \<open>Implementation of the proof forest\<close>
 
-function (domintros) add_edge :: "nat list \<Rightarrow> nat \<Rightarrow> nat \<Rightarrow> nat list"
-  where
-"add_edge pf e e' = (if pf ! e = e then (pf[e := e']) else add_edge (pf[e := e']) (pf ! e) e)"
+function (domintros) add_edge :: "nat list \<Rightarrow> nat \<Rightarrow> nat \<Rightarrow> nat list" where
+  "add_edge pf e e' = (if pf ! e = e then pf[e := e'] else add_edge (pf[e := e']) (pf ! e) e)"
   by pat_completeness auto
 
-lemma add_edge_rel: "rep_of_rel (l, x) (l, y) \<longleftrightarrow> add_edge_rel (l[y := y'], x, y) (l, y, y')" 
+lemma add_edge_rel:
+  "rep_of_rel (l, x) (l, y) \<longleftrightarrow> add_edge_rel (l[y := y'], x, y) (l, y, y')" 
 proof
   show "rep_of_rel (l, x) (l, y) \<Longrightarrow> add_edge_rel (l[y := y'], x, y) (l, y, y')"
-    by (induction "(l, x)" "(l, y)" rule: rep_of_rel.induct)(auto simp add: add_edge_rel.intros)
+    by (induction "(l, x)" "(l, y)" rule: rep_of_rel.induct)
+       (auto simp add: add_edge_rel.intros)
 next
   show "add_edge_rel (l[y := y'], x, y) (l, y, y') \<Longrightarrow> rep_of_rel (l, x) (l, y)"
-    by (induction "(l[y := y'], x, y)" "(l, y, y')" rule: add_edge_rel.induct) (auto simp add: rep_of_rel.intros)
+    by (induction "(l[y := y'], x, y)" "(l, y, y')" rule: add_edge_rel.induct)
+       (auto simp add: rep_of_rel.intros)
 qed
 
-function (domintros) add_label :: "pending_equation option list \<Rightarrow> nat list \<Rightarrow> nat \<Rightarrow> pending_equation \<Rightarrow> pending_equation option list"
-  where
-"add_label pfl pf e lbl = (if pf ! e = e then (pfl[e := Some lbl]) else add_label (pfl[e := Some lbl]) pf (pf ! e) (the (pfl ! e)))"
+function (domintros) add_label ::
+  "pending_equation option list \<Rightarrow> nat list \<Rightarrow> nat \<Rightarrow> pending_equation
+  \<Rightarrow> pending_equation option list" where
+  "add_label pfl pf e lbl =
+    (if pf ! e = e
+      then pfl[e := Some lbl]
+      else add_label (pfl[e := Some lbl]) pf (pf ! e) (the (pfl ! e)))"
   by pat_completeness auto
 
-fun propagate_loop
-  where
-"propagate_loop rep_b (u1 # urest) 
-\<lparr>cc_list = l, use_list = u, lookup = t, pending = pe, proof_forest = pf, pf_labels = pfl, input = ip\<rparr>
-=
-  propagate_loop rep_b urest (
-    if (lookup_Some t l u1)
-    then 
-      \<lparr>cc_list = l, use_list = u, lookup = t, 
-            pending = link_to_lookup t l u1#pe,
-            proof_forest = pf, pf_labels = pfl, input = ip\<rparr>
-    else
-      \<lparr>cc_list = l,
-            use_list = u[rep_b := u1 # (u ! rep_b)],
-            lookup = update_lookup t l u1, 
-            pending = pe, proof_forest = pf, pf_labels = pfl, input = ip\<rparr>
-)"
+fun propagate_loop where
+  "propagate_loop rep_b (u1 # urest) cc_state =
+    propagate_loop rep_b urest (
+      if lookup_Some (lookup cc_state) (cc_list cc_state) u1
+      then cc_state \<lparr> pending := link_to_lookup (lookup cc_state) (cc_list cc_state) u1 # pending cc_state \<rparr>
+      else cc_state \<lparr> use_list := (use_list cc_state)[rep_b := u1 # (use_list cc_state ! rep_b)]
+                    , lookup := update_lookup (lookup cc_state) (cc_list cc_state) u1
+                    \<rparr>
+      )"
 | "propagate_loop _ [] cc = cc"
 
-abbreviation propagate_step
-  where 
-"propagate_step l u t pe pf pfl ip a b eq \<equiv> 
-  propagate_loop (rep_of l b) (u ! rep_of l a)
-    \<lparr>cc_list = ufa_union l a b, 
-    use_list = u[rep_of l a := []], 
-    lookup = t, 
-    pending = pe,
-    proof_forest = add_edge pf a b, 
-    pf_labels = add_label pfl pf a eq, 
-    input = ip\<rparr>"
+abbreviation propagate_step where 
+"propagate_step cc_state a b eq \<equiv> 
+  propagate_loop (rep_of (cc_list cc_state) b) (use_list cc_state ! rep_of (cc_list cc_state) a)
+    (cc_state 
+      \<lparr> cc_list := ufa_union (cc_list cc_state) a b 
+      , use_list := (use_list cc_state)[rep_of (cc_list cc_state) a := []] 
+      , proof_forest := add_edge (proof_forest cc_state) a b 
+      , pf_labels := add_label (pf_labels cc_state) (proof_forest cc_state) a eq 
+      \<rparr>)"
 
-function (domintros) propagate :: "congruence_closure \<Rightarrow> congruence_closure"
-  where
-"propagate \<lparr>cc_list = l, use_list = u, lookup = t, pending = [], proof_forest = pf, pf_labels = pfl, input = ip\<rparr> = 
-\<lparr>cc_list = l, use_list = u, lookup = t, pending = [], proof_forest = pf, pf_labels = pfl, input = ip\<rparr>"
-| "propagate 
-\<lparr>cc_list = l, use_list = u, lookup = t, pending = (eq # pe), proof_forest = pf, pf_labels = pfl, input = ip\<rparr> = 
-(let a = left eq; b = right eq in
-  (if rep_of l a = rep_of l b 
-    then propagate \<lparr>cc_list = l, use_list = u, lookup = t, pending = pe, proof_forest = pf, pf_labels = pfl, input = ip\<rparr>
-    else
-      propagate (propagate_step l u t pe pf pfl ip a b eq)
-))"
+function (domintros) propagate :: "cc_state \<Rightarrow> cc_state" where
+"propagate cc_state =
+  (case pending cc_state of
+    [] \<Rightarrow> cc_state
+  | (eq # pe) \<Rightarrow> 
+    let a = left eq; b = right eq in
+      (if rep_of (cc_list cc_state) a = rep_of (cc_list cc_state) b 
+        then propagate (cc_state \<lparr> pending := pe \<rparr>)
+        else propagate (propagate_step (cc_state \<lparr> pending := pe \<rparr>) a b eq))
+  )"
   by pat_completeness auto
 
-lemma propagate_simps1[simp]:
-  assumes "propagate_dom cc"
-"pending cc = []"
-shows "propagate cc = cc"
+lemma propagate_if_pending_eq_Nil[simp]:
+  assumes "propagate_dom cc" "pending cc = []"
+  shows "propagate cc = cc"
   using assms propagate.psimps propagate.pelims by fastforce
 
-lemma propagate_simps2[simp]:
-  assumes "propagate_dom \<lparr>cc_list = l, use_list = u, lookup = t, pending = (eq # pe), proof_forest = pf, pf_labels = pfl, input = ip\<rparr>"
-"rep_of l (left eq) = rep_of l (right eq)"
-shows "propagate 
-\<lparr>cc_list = l, use_list = u, lookup = t, pending = (eq # pe), proof_forest = pf, pf_labels = pfl, input = ip\<rparr>
- = propagate \<lparr>cc_list = l, use_list = u, lookup = t, pending = pe, proof_forest = pf, pf_labels = pfl, input = ip\<rparr>"
+lemma propagate_if_pending_eq_Cons_and_rep_of_eq[simp]:
+  assumes "propagate_dom cc_state"
+      and "pending cc_state = eq # pe"
+      and "rep_of (cc_list cc_state) (left eq) = rep_of (cc_list cc_state) (right eq)"
+    shows "propagate cc_state = propagate (cc_state \<lparr> pending := pe \<rparr>)"
   using assms propagate.psimps unfolding Let_def by auto
 
-lemma propagate_simps3[simp]:
-  assumes "propagate_dom \<lparr>cc_list = l, use_list = u, lookup = t, pending = (eq # pe), proof_forest = pf, pf_labels = pfl, input = ip\<rparr>"
-"rep_of l (left eq) \<noteq> rep_of l (right eq)"
-shows "propagate 
-\<lparr>cc_list = l, use_list = u, lookup = t, pending = (eq # pe), proof_forest = pf, pf_labels = pfl, input = ip\<rparr>
- = propagate (propagate_step l u t pe pf pfl ip (left eq) (right eq) eq)"
-  using assms propagate.psimps unfolding Let_def by auto
+lemma propagate_if_pending_eq_Cons_and_rep_of_neq[simp]:
+  assumes "propagate_dom cc_state"
+      and "pending cc_state = eq # pe"
+      and "rep_of (cc_list cc_state) (left eq) \<noteq> rep_of (cc_list cc_state) (right eq)"
+    shows "propagate cc_state
+          = propagate (propagate_step (cc_state \<lparr> pending := pe \<rparr>) (left eq) (right eq) eq)"
+  using assms propagate.psimps unfolding Let_def by simp
 
-fun merge :: "congruence_closure \<Rightarrow> equation \<Rightarrow> congruence_closure"
+term list_update
+fun merge :: "cc_state \<Rightarrow> equation \<Rightarrow> cc_state"
   where 
-"merge \<lparr>cc_list = l, use_list = u, lookup = t, pending = pe, proof_forest = pf, pf_labels = pfl, input = ip\<rparr> 
-(a \<approx> b) = 
-  propagate 
-    \<lparr>cc_list = l, use_list = u, lookup = t, pending = One (a \<approx> b)#pe, proof_forest = pf, pf_labels = pfl, input = insert (a \<approx> b) ip\<rparr>"
-
-| "merge \<lparr>cc_list = l, use_list = u, lookup = t, pending = pe, proof_forest = pf, pf_labels = pfl, input = ip\<rparr> 
-(F a\<^sub>1 a\<^sub>2 \<approx> a) = 
-(if (lookup_Some t l (F a\<^sub>1 a\<^sub>2 \<approx> a))
-  then propagate \<lparr>cc_list = l, use_list = u, lookup = t, 
-            pending = link_to_lookup t l (F a\<^sub>1 a\<^sub>2 \<approx> a)#pe, proof_forest = pf, pf_labels = pfl, input = insert (F a\<^sub>1 a\<^sub>2 \<approx> a) ip\<rparr>
-  else \<lparr>cc_list = l, 
-          use_list = (u[rep_of l a\<^sub>1 := (F a\<^sub>1 a\<^sub>2 \<approx> a)#(u ! rep_of l a\<^sub>1)])[rep_of l a\<^sub>2 := (F a\<^sub>1 a\<^sub>2 \<approx> a)#(u ! rep_of l a\<^sub>2)], 
-          lookup = update_lookup t l (F a\<^sub>1 a\<^sub>2 \<approx> a), 
-          pending = pe, proof_forest = pf, pf_labels = pfl, input = insert (F a\<^sub>1 a\<^sub>2 \<approx> a) ip\<rparr>
-)"
+  "merge cc_state (a \<approx> b) = propagate (cc_state\<lparr> pending := One (a \<approx> b) # pending cc_state
+                                               , input := insert (a \<approx> b) (input cc_state)
+                                               \<rparr>)"
+| "merge \<lparr> cc_list = l , use_list = u, lookup = t, pending = pe
+         , proof_forest = pf, pf_labels = pfl
+         , input = ip
+         \<rparr> 
+        (F a\<^sub>1 a\<^sub>2 \<approx> a) = 
+  (if lookup_Some t l (F a\<^sub>1 a\<^sub>2 \<approx> a)
+    then propagate \<lparr> cc_list = l, use_list = u, lookup = t
+                   , pending = link_to_lookup t l (F a\<^sub>1 a\<^sub>2 \<approx> a) # pe
+                   , proof_forest = pf, pf_labels = pfl
+                   , input = insert (F a\<^sub>1 a\<^sub>2 \<approx> a) ip
+                   \<rparr>
+    else
+      let rep_a\<^sub>1 = rep_of l a\<^sub>1; rep_a\<^sub>2 = rep_of l a\<^sub>2 in
+        \<lparr> cc_list = l
+        , use_list = u[rep_a\<^sub>1 := (F a\<^sub>1 a\<^sub>2 \<approx> a) # (u ! rep_a\<^sub>1), rep_a\<^sub>2 := (F a\<^sub>1 a\<^sub>2 \<approx> a) # (u ! rep_a\<^sub>2)]
+        , lookup = update_lookup t l (F a\<^sub>1 a\<^sub>2 \<approx> a)
+        , pending = pe
+        , proof_forest = pf, pf_labels = pfl
+        , input = insert (F a\<^sub>1 a\<^sub>2 \<approx> a) ip
+        \<rparr>)"
 
 text \<open>The input must be a valid index (a < nr_vars cc \<and> b < nr_vars cc)\<close>
-fun are_congruent :: "congruence_closure \<Rightarrow> equation \<Rightarrow> bool"
-  where
-"are_congruent \<lparr>cc_list = l, use_list = u, lookup = t, pending = pe, proof_forest = pf, pf_labels = pfl, input = ip\<rparr> (a \<approx> b) = 
-    (rep_of l a = rep_of l b)"
-| "are_congruent \<lparr>cc_list = l, use_list = u, lookup = t, pending = pe, proof_forest = pf, pf_labels = pfl, input = ip\<rparr> (F a\<^sub>1 a\<^sub>2 \<approx> a) = 
-    (case lookup_entry t l a\<^sub>1 a\<^sub>2 of
-      Some (F b\<^sub>1 b\<^sub>2 \<approx> b) \<Rightarrow> (rep_of l a = rep_of l b)
-    | None \<Rightarrow> False
-)"
+fun are_congruent :: "cc_state \<Rightarrow> equation \<Rightarrow> bool" where
+  "are_congruent cc_state (a \<approx> b) \<longleftrightarrow> rep_of (cc_list cc_state) a = rep_of (cc_list cc_state) b" 
+| "are_congruent cc_state (F a\<^sub>1 a\<^sub>2 \<approx> a) = 
+    (case lookup_entry (lookup cc_state) (cc_list cc_state) a\<^sub>1 a\<^sub>2 of
+      Some (F b\<^sub>1 b\<^sub>2 \<approx> b) \<Rightarrow> rep_of (cc_list cc_state) a = rep_of (cc_list cc_state) b
+    | None \<Rightarrow> False)"
 
 lemma are_congruent_simp:
-"are_congruent cc (a \<approx> b) = (rep_of (cc_list cc) a = rep_of (cc_list cc) b)"
-  by (metis are_congruent.simps(1) congruence_closure.surjective old.unit.exhaust)
-
+  "are_congruent cc (a \<approx> b) \<longleftrightarrow> rep_of (cc_list cc) a = rep_of (cc_list cc) b"
+  by (cases "(cc, a \<approx> b)" rule: are_congruent.cases) simp_all
+  
 text \<open>For the initialisation of the congruence closure algorithm.\<close>
 abbreviation 
-"initial_cc n \<equiv> \<lparr>cc_list = [0..<n], use_list = replicate n [], lookup = replicate n (replicate n None),
-                  pending = [], proof_forest = [0..<n], pf_labels = replicate n None, input = {}\<rparr>"
+  "initial_cc n \<equiv> \<lparr> cc_list = [0..<n]
+                  , use_list = replicate n []
+                  , lookup = replicate n (replicate n None)
+                  , pending = []
+                  , proof_forest = [0..<n]
+                  , pf_labels = replicate n None
+                  , input = {}
+                  \<rparr>"
 
 end
